theories/Irrelevance.v
@@ -1,12 +1,14 @@
 From LogRel.AutoSubst Require Import core unscoped Ast.
 From LogRel Require Import Utils BasicAst Notations Context Untyped Weakening GenericTyping LogicalRelation Reduction LRInduction ShapeView Reflexivity.
 
+Set Universe Polymorphism.
+
 Section Irrelevances.
 Context `{GenericTypingProperties}.
 
-
 Section ΠIrrelevanceLemmas.
-Context Γ A A' (ΠA : PiRedTy Γ A) (ΠA' : PiRedTy Γ A') 
+Universe u.
+Context Γ A A' (ΠA : PiRedTy@{u} Γ A) (ΠA' : PiRedTy@{u} Γ A') 
   (dom := PiRedTy.dom ΠA)
   (dom' := PiRedTy.dom ΠA')
   (domRed := (@PiRedTy.domRed _ _ _ _ _ _ _ ΠA))
@@ -17,25 +19,27 @@ Context Γ A A' (ΠA : PiRedTy Γ A) (ΠA' : PiRedTy Γ A')
   (codRed' := (@PiRedTy.codRed _ _ _ _ _ _ _ ΠA'))
   (eqPi : [Γ |- tProd (PiRedTy.na ΠA) dom cod ≅ tProd (PiRedTy.na ΠA') dom' cod']).
 
+Notation "A <≈> B" := (prod@{u u} (A -> B) (B -> A)) (at level 90).
+
 Lemma ΠIrrelevanceTyEq  :
   (forall (Δ : context) (ρ : Δ ≤ Γ) (h : [  |- Δ]),
   [× (forall B : term,
-      [domRed Δ ρ h | Δ ||- dom⟨ρ⟩ ≅ B] <~> [domRed' Δ ρ h | Δ ||- dom'⟨ρ⟩ ≅ B]),
+      [domRed Δ ρ h | Δ ||- dom⟨ρ⟩ ≅ B] <≈> [domRed' Δ ρ h | Δ ||- dom'⟨ρ⟩ ≅ B]),
     (forall t : term,
-      [domRed Δ ρ h | Δ ||- t : dom⟨ρ⟩] <~> [domRed' Δ ρ h | Δ ||- t : dom'⟨ρ⟩]) &
+      [domRed Δ ρ h | Δ ||- t : dom⟨ρ⟩] <≈> [domRed' Δ ρ h | Δ ||- t : dom'⟨ρ⟩]) &
     (forall t u : term,
-      [domRed Δ ρ h | Δ ||- t ≅ u : dom⟨ρ⟩ ] <~> [domRed' Δ ρ h | Δ ||- t ≅ u : dom'⟨ρ⟩])]) ->
+      [domRed Δ ρ h | Δ ||- t ≅ u : dom⟨ρ⟩ ] <≈> [domRed' Δ ρ h | Δ ||- t ≅ u : dom'⟨ρ⟩])]) ->
   (forall (Δ : context) (ρ : Δ ≤ Γ) (a : term) (h : [  |- Δ])
       (ha : [domRed Δ ρ h | Δ ||- a : dom⟨ρ⟩])
       (ha' : [domRed' Δ ρ h | Δ ||- a : dom'⟨ρ⟩]),
   [× (forall B : term,
-      [codRed Δ a ρ h ha | Δ ||- cod[a .: (ρ >> tRel)] ≅ B] <~>
+      [codRed Δ a ρ h ha | Δ ||- cod[a .: (ρ >> tRel)] ≅ B] <≈>
       [codRed' Δ a ρ h ha' | Δ ||- cod'[a .: (ρ >> tRel)] ≅ B]),
     (forall t : term,
-      [codRed Δ a ρ h ha | Δ ||- t : cod[a .: (ρ >> tRel)] ] <~>
+      [codRed Δ a ρ h ha | Δ ||- t : cod[a .: (ρ >> tRel)] ] <≈>
       [codRed' Δ a ρ h ha' | Δ ||- t : cod'[a .: (ρ >> tRel)]]) &
     (forall t u : term,
-      [codRed Δ a ρ h ha | Δ ||- t ≅ u : cod[a .: (ρ >> tRel)]] <~>
+      [codRed Δ a ρ h ha | Δ ||- t ≅ u : cod[a .: (ρ >> tRel)]] <≈>
       [codRed' Δ a ρ h ha' | Δ ||- t ≅ u : cod'[a .: (ρ >> tRel)] ])]) ->
   forall B, [Γ ||-Π A ≅ B | ΠA] -> [Γ ||-Π A' ≅ B | ΠA'].
 Proof.
@@ -57,22 +61,22 @@ Qed.
 Lemma ΠIrrelevanceTm  :
   (forall (Δ : context) (ρ : Δ ≤ Γ) (h : [  |- Δ]),
   [× (forall B : term,
-      [domRed Δ ρ h | Δ ||- dom⟨ρ⟩ ≅ B] <~> [domRed' Δ ρ h | Δ ||- dom'⟨ρ⟩ ≅ B]),
+      [domRed Δ ρ h | Δ ||- dom⟨ρ⟩ ≅ B] <≈> [domRed' Δ ρ h | Δ ||- dom'⟨ρ⟩ ≅ B]),
     (forall t : term,
-      [domRed Δ ρ h | Δ ||- t : dom⟨ρ⟩] <~> [domRed' Δ ρ h | Δ ||- t : dom'⟨ρ⟩]) &
+      [domRed Δ ρ h | Δ ||- t : dom⟨ρ⟩] <≈> [domRed' Δ ρ h | Δ ||- t : dom'⟨ρ⟩]) &
     (forall t u : term,
-      [domRed Δ ρ h | Δ ||- t ≅ u : dom⟨ρ⟩ ] <~> [domRed' Δ ρ h | Δ ||- t ≅ u : dom'⟨ρ⟩])]) ->
+      [domRed Δ ρ h | Δ ||- t ≅ u : dom⟨ρ⟩ ] <≈> [domRed' Δ ρ h | Δ ||- t ≅ u : dom'⟨ρ⟩])]) ->
   (forall (Δ : context) (ρ : Δ ≤ Γ) (a : term) (h : [  |- Δ])
       (ha : [domRed Δ ρ h | Δ ||- a : dom⟨ρ⟩])
       (ha' : [domRed' Δ ρ h | Δ ||- a : dom'⟨ρ⟩]),
   [× (forall B : term,
-      [codRed Δ a ρ h ha | Δ ||- cod[a .: (ρ >> tRel)] ≅ B] <~>
+      [codRed Δ a ρ h ha | Δ ||- cod[a .: (ρ >> tRel)] ≅ B] <≈>
       [codRed' Δ a ρ h ha' | Δ ||- cod'[a .: (ρ >> tRel)] ≅ B]),
     (forall t : term,
-      [codRed Δ a ρ h ha | Δ ||- t : cod[a .: (ρ >> tRel)] ] <~>
+      [codRed Δ a ρ h ha | Δ ||- t : cod[a .: (ρ >> tRel)] ] <≈>
       [codRed' Δ a ρ h ha' | Δ ||- t : cod'[a .: (ρ >> tRel)]]) &
     (forall t u : term,
-      [codRed Δ a ρ h ha | Δ ||- t ≅ u : cod[a .: (ρ >> tRel)]] <~>
+      [codRed Δ a ρ h ha | Δ ||- t ≅ u : cod[a .: (ρ >> tRel)]] <≈>
       [codRed' Δ a ρ h ha' | Δ ||- t ≅ u : cod'[a .: (ρ >> tRel)] ])]) ->
   forall t, [Γ ||-Π t : A | ΠA] -> [Γ ||-Π t : A' | ΠA'].
 Proof.
@@ -96,22 +100,22 @@ Defined.
 Lemma ΠIrrelevanceTmEq  :
   (forall (Δ : context) (ρ : Δ ≤ Γ) (h : [  |- Δ]),
   [× (forall B : term,
-      [domRed Δ ρ h | Δ ||- dom⟨ρ⟩ ≅ B] <~> [domRed' Δ ρ h | Δ ||- dom'⟨ρ⟩ ≅ B]),
+      [domRed Δ ρ h | Δ ||- dom⟨ρ⟩ ≅ B] <≈> [domRed' Δ ρ h | Δ ||- dom'⟨ρ⟩ ≅ B]),
     (forall t : term,
-      [domRed Δ ρ h | Δ ||- t : dom⟨ρ⟩] <~> [domRed' Δ ρ h | Δ ||- t : dom'⟨ρ⟩]) &
+      [domRed Δ ρ h | Δ ||- t : dom⟨ρ⟩] <≈> [domRed' Δ ρ h | Δ ||- t : dom'⟨ρ⟩]) &
     (forall t u : term,
-      [domRed Δ ρ h | Δ ||- t ≅ u : dom⟨ρ⟩ ] <~> [domRed' Δ ρ h | Δ ||- t ≅ u : dom'⟨ρ⟩])]) ->
+      [domRed Δ ρ h | Δ ||- t ≅ u : dom⟨ρ⟩ ] <≈> [domRed' Δ ρ h | Δ ||- t ≅ u : dom'⟨ρ⟩])]) ->
   (forall (Δ : context) (ρ : Δ ≤ Γ) (a : term) (h : [  |- Δ])
       (ha : [domRed Δ ρ h | Δ ||- a : dom⟨ρ⟩])
       (ha' : [domRed' Δ ρ h | Δ ||- a : dom'⟨ρ⟩]),
   [× (forall B : term,
-      [codRed Δ a ρ h ha | Δ ||- cod[a .: (ρ >> tRel)] ≅ B] <~>
+      [codRed Δ a ρ h ha | Δ ||- cod[a .: (ρ >> tRel)] ≅ B] <≈>
       [codRed' Δ a ρ h ha' | Δ ||- cod'[a .: (ρ >> tRel)] ≅ B]),
     (forall t : term,
-      [codRed Δ a ρ h ha | Δ ||- t : cod[a .: (ρ >> tRel)] ] <~>
+      [codRed Δ a ρ h ha | Δ ||- t : cod[a .: (ρ >> tRel)] ] <≈>
       [codRed' Δ a ρ h ha' | Δ ||- t : cod'[a .: (ρ >> tRel)]]) &
     (forall t u : term,
-      [codRed Δ a ρ h ha | Δ ||- t ≅ u : cod[a .: (ρ >> tRel)]] <~>
+      [codRed Δ a ρ h ha | Δ ||- t ≅ u : cod[a .: (ρ >> tRel)]] <≈>
       [codRed' Δ a ρ h ha' | Δ ||- t ≅ u : cod'[a .: (ρ >> tRel)] ])]) ->
   forall t u, [Γ ||-Π t ≅ u : A | ΠA] -> [Γ ||-Π t ≅ u : A' | ΠA'].
 Proof.
@@ -129,13 +133,19 @@ Qed.
 
 End ΠIrrelevanceLemmas.
 
+Section LRIrrelevant.
+Universe i j k.
 
-Theorem LRIrrelevant Γ A A' {lA eqTyA redTmA eqTmA lA' eqTyA' redTmA' eqTmA'}
-    (lrA : LogRel lA Γ A eqTyA redTmA eqTmA) (lrA' : LogRel lA' Γ A' eqTyA' redTmA' eqTmA') :
+Notation "A <≈> B" := (prod@{j j} (A -> B) (B -> A)) (at level 90).
+
+Theorem LRIrrelevant Γ A A' {lA lA'}
+  {eqTyA redTmA eqTyA' redTmA' : term -> Type@{j}}
+  {eqTmA eqTmA' : term -> term -> Type@{j}}
+    (lrA : LogRel@{i j k} lA Γ A eqTyA redTmA eqTmA) (lrA' : LogRel@{i j k} lA' Γ A' eqTyA' redTmA' eqTmA') :
     eqTyA A' ->
-    [× forall B, eqTyA B <~> eqTyA' B ,
-    forall t, redTmA t <~> redTmA' t &
-    forall t u, eqTmA t u <~> eqTmA' t u ].
+    [× forall B, eqTyA B <≈> eqTyA' B ,
+    forall t, redTmA t <≈> redTmA' t &
+    forall t u, eqTmA t u <≈> eqTmA' t u ].
 Proof.
   intros he.
   set (s := ShapeViewConv lrA lrA' he).
@@ -158,11 +168,14 @@ Proof.
       all: eassumption.
   - destruct lrA' as [|? A' neA'|] ; try solve [destruct s] ; clear s.
     destruct he as [AA], neA' as [AA'] ; cbn in *.
-    assert (AA' = AA) as ->.
+    assert (AA' = AA) as eqAA'.
     {
       all: eapply whredty_det ; econstructor ; [idtac |now econstructor| idtac |now econstructor].
       all: gen_typing.
     }
+    revert red1 ne1 eq1. pattern AA'.
+    set (P := fun _ => _). apply (tr P (eq_sym eqAA')). subst P; cbn.
+    intros red1 ne1 eq1.
     assert [Γ |- ty ≅ AA] as convtAA by gen_typing.
     split.
     + intros ?.
@@ -172,7 +185,7 @@ Proof.
       all: cbn in *.
       all: try eauto.
       2: etransitivity ; eassumption.
-      etransitivity ; [symmetry|..] ; eassumption.
+      clear eq1; etransitivity ; [symmetry|..]; eassumption.
     + intros ?.
       split.
       2: symmetry in convtAA.
@@ -201,13 +214,13 @@ Proof.
       (ha' : [domRed0 Δ ρ h | Δ ||- a : dom1⟨ρ⟩]),
       [×
         (forall B,
-          [codRed Δ a ρ h ha | Δ ||- cod[a .: (ρ >> tRel)] ≅ B] <~>
+          [codRed Δ a ρ h ha | Δ ||- cod[a .: (ρ >> tRel)] ≅ B] <≈>
           [codRed0 Δ a ρ h ha' | Δ ||- cod1[a .: (ρ >> tRel)] ≅ B]),
         (forall t,
-          [codRed Δ a ρ h ha | Δ ||- t : cod[a .: (ρ >> tRel)]] <~>
+          [codRed Δ a ρ h ha | Δ ||- t : cod[a .: (ρ >> tRel)]] <≈>
           [codRed0 Δ a ρ h ha' | Δ ||- t : cod1[a .: (ρ >> tRel)]]) &
       (forall t u,
-        [codRed Δ a ρ h ha | Δ ||- t ≅ u : cod[a .: (ρ >> tRel)]] <~>
+        [codRed Δ a ρ h ha | Δ ||- t ≅ u : cod[a .: (ρ >> tRel)]] <≈>
         [codRed0 Δ a ρ h ha' | Δ ||- t ≅ u : cod1[a .: (ρ >> tRel)]])
       ]).
     {
@@ -245,6 +258,138 @@ Proof.
       * do 2 split ; intros.
         all: now eapply IHcod_ ; eauto.
 Qed.
+
+
+End LRIrrelevant.
+
+Section LRIrrelevant0.
+Universe i j.
+
+Notation "A <≈> B" := (prod@{i i} (A -> B) (B -> A)) (at level 90).
+
+Theorem LRIrrelevant0 Γ A A'
+  {eqTyA redTmA eqTyA' redTmA' : term -> Type@{i}}
+  {eqTmA eqTmA' : term -> term -> Type@{i}}
+    (lrA : LogRel0@{i j} Γ A eqTyA redTmA eqTmA) (lrA' : LogRel0@{i j} Γ A' eqTyA' redTmA' eqTmA') :
+    eqTyA A' ->
+    [× forall B, eqTyA B <≈> eqTyA' B ,
+    forall t, redTmA t <≈> redTmA' t &
+    forall t u, eqTmA t u <≈> eqTmA' t u ].
+Proof.
+  intros he.
+  set (s := ShapeViewConv0 lrA lrA' he).
+  revert A' eqTyA' redTmA' eqTmA' lrA' he s.
+  pattern Γ, A, eqTyA, redTmA, eqTmA, lrA.
+  match goal with [|- ?X _ _ _ _ _ _] => pose (P := X) end.
+  eapply LR_rect0; clear Γ A eqTyA redTmA eqTmA lrA; subst P.
+  (* induction lrA as [? [? []] | ? ? [] | ? A [] [] IHdom IHcod] *)
+  (*   in A', eqTyA', eqTmA', redTmA', lrA', he, s |- *. *)
+  - intros Γ A neA A' eqTyA' redTmA' eqTmA' lrA'.
+    revert neA; pattern Γ, A', eqTyA', redTmA',  eqTmA', lrA'.
+    match goal with [|- ?X _ _ _ _ _ _] => pose (P := X) end.
+    eapply LR_rect0; clear Γ A' eqTyA' redTmA'  eqTmA' lrA'; subst P.
+    2: intros ???????? [].
+    intros Γ A' [AA' red1 ne1 eq1] [ty red0 ne0 eq0] [AA] _; cbn in *.
+    assert (AA' = AA) as eqAA'.
+    {
+      eapply whredty_det; econstructor ; [idtac |now econstructor| idtac |now econstructor].
+      all: gen_typing.
+    }
+    revert red1 ne1 eq1. pattern AA'.
+    set (P := fun _ => _). apply (tr P (eq_sym eqAA')). subst P; cbn.
+    intros red1 ne1 eq1.
+    assert [Γ |- ty ≅ AA] as convtAA by gen_typing.
+    split.
+    + intros ?.
+      split.
+      all: intros [].
+      all: econstructor.
+      all: cbn in *.
+      all: try eauto.
+      2: etransitivity ; eassumption.
+      clear eq1; etransitivity ; [symmetry|..]; eassumption.
+    + intros ?.
+      split.
+      2: symmetry in convtAA.
+      all: intros [].
+      all: econstructor ; cbn in *.
+      all: try eauto.
+      1,3: eapply wfredtm_conv ; eassumption.
+      all: gen_typing.
+    + intros ? ?.
+      split.
+      2: symmetry in convtAA.
+      all: intros [].
+      all: econstructor.
+      all: cbn in *.
+      1-2,6-7: eapply wfredtm_conv ; eassumption.
+      1-2,4-5: eassumption.
+      all: now gen_typing.
+  - intros Γ A ΠA ΠAad IHdom IHcod A' eqTyA' redTmA' eqTmA' lrA'.
+    revert ΠA ΠAad IHdom IHcod.
+    pattern Γ, A', eqTyA', redTmA',  eqTmA', lrA'.
+    match goal with [|- ?X _ _ _ _ _ _] => pose (P := X) end.
+    eapply LR_rect0; clear Γ A' eqTyA' redTmA'  eqTmA' lrA'; subst P.
+    1: intros ???????? [].
+    intros Γ A' [] [] _ _ [] [] IHdom IHcod [].
+    cbn -[subst1] in *.
+    assert (tProd na dom cod = tProd na1 dom1 cod1) as ePi
+      by (eapply whredty_det ; gen_typing).
+    inversion ePi ; subst ; clear ePi.
+    pose proof (IHdom_ := fun Δ ρ h => IHdom Δ ρ h _ _ _ _ (domAd Δ ρ h) (domRed1 Δ ρ h)).
+    assert (IHcod_ : forall Δ a (ρ : Δ ≤ Γ) (h : [|- Δ])
+      (ha : [domRed Δ ρ h | Δ ||- a : dom1⟨ρ⟩])
+      (ha' : [domRed0 Δ ρ h | Δ ||- a : dom0⟨ρ⟩]),
+      [×
+        (forall B,
+          [codRed0 Δ a ρ h ha' | Δ ||- cod0[a .: (ρ >> tRel)] ≅ B] <≈>
+          [codRed Δ a ρ h ha | Δ ||- cod1[a .: (ρ >> tRel)] ≅ B]),
+        (forall t,
+          [codRed0 Δ a ρ h ha' | Δ ||- t : cod0[a .: (ρ >> tRel)]] <≈>
+          [codRed Δ a ρ h ha | Δ ||- t : cod1[a .: (ρ >> tRel)]]) &
+      (forall t u,
+        [codRed0 Δ a ρ h ha' | Δ ||- t ≅ u : cod0[a .: (ρ >> tRel)]] <≈>
+        [codRed Δ a ρ h ha | Δ ||- t ≅ u : cod1[a .: (ρ >> tRel)]])
+      ]).
+    {
+      intros.
+      eapply IHcod.
+      1: eapply codAd.
+      eauto.
+    }
+    split.
+    + split ; intros.
+      all: eapply ΠIrrelevanceTyEq.
+      4,8: eassumption. 
+      1,4: assumption + now symmetry.
+      1-2: now eauto.
+      * do 2 split ; intros.
+        all: now eapply IHdom_ ; eauto.
+      * do 2 split ; intros.
+        all: now eapply IHcod_ ; eauto.
+    + split ; intros.
+      all: eapply ΠIrrelevanceTm.
+      4,8: eassumption. 
+      1,4: assumption + now symmetry.
+      1-2: now eauto.
+      * do 2 split ; intros.
+        all: now eapply IHdom_ ; eauto.
+      * do 2 split ; intros.
+        all: now eapply IHcod_ ; eauto.
+    + split ; intros.
+      all: eapply ΠIrrelevanceTmEq.
+      4,8: eassumption. 
+      1,4: assumption + now symmetry.
+      1-2: now eauto.
+      * do 2 split ; intros.
+        all: now eapply IHdom_ ; eauto.
+      * do 2 split ; intros.
+        all: now eapply IHcod_ ; eauto.
+Qed.
+
+
+End LRIrrelevant0.
+
 
 Corollary TyEqIrrelevant Γ A {lA eqTyA redTmA eqTmA lA' eqTyA' redTmA' eqTmA'}
   (lrA : LogRel lA Γ A eqTyA redTmA eqTmA) (lrA' : LogRel lA' Γ A eqTyA' redTmA' eqTmA') :
@@ -347,15 +492,33 @@ Proof.
   now eapply TmEqRedConv.
 Qed.
 
+Corollary TyEqSym0 Γ A A' {eqTyA redTmA eqTmA eqTyA' redTmA' eqTmA'}
+  (lrA : LogRel0 Γ A eqTyA redTmA eqTmA) (lrA' : LogRel0 Γ A' eqTyA' redTmA' eqTmA') :
+  eqTyA A' -> eqTyA' A.
+Proof.
+  intros.
+  apply (LRIrrelevant0 _ _ _ lrA lrA').
+  1: eauto.
+  now eapply LRTyEqRefl0.
+Qed.
+
+Corollary LRTyEqSym0 Γ A A' (lrA : [Γ ||-<0> A]) (lrA' : [Γ ||-<0> A']) :
+  [Γ ||-<0> A ≅ A' | lrA] -> [Γ ||-<0> A' ≅ A | lrA'].
+Proof.
+  destruct lrA, lrA'.
+  cbn in *.
+  now eapply TyEqSym0.
+Qed.
+
 Set Printing Primitive Projection Parameters.
 
-Lemma LRTmEqSym lA Γ A (lrA : [Γ ||-<lA> A]) : forall t u,
+Lemma LRTmEqSym@{i j k} lA Γ A (lrA : [LogRel@{i j k} lA | Γ ||- A]) : forall t u,
   [Γ ||-<lA> t ≅ u : A |lrA] -> [Γ ||-<lA> u ≅ t : A |lrA].
 Proof.
   pattern lA, Γ, A, lrA. apply LR_rect_TyUr.
   - intros * []. unshelve econstructor; try eassumption.
     1: symmetry; eassumption.
-    eapply LRTyEqSym. exact relEq.
+    eapply LRTyEqSym0. exact relEq.
   - intros * []. unshelve econstructor.
     3,4: eassumption.
     1,2: eassumption.
