theories/Notations.v
@@ -206,6 +206,15 @@ Reserved Notation "[ Γ ||-< l >  t : A | R ]" (at level 0, Γ, l, t, A, R at le
 (* The terms t and u are reducibly convertible at type A and level l in Γ, given the proof R that A is reducible *)
 Reserved Notation "[ Γ ||-< l > t ≅ u : A | R ]" (at level 0, Γ, l, t, u, A, R at level 50).
 
+(* The type A is reducible in Γ at level 0*)
+Reserved Notation "[ Γ ||-<0>  A ]" (at level 0, Γ, A at level 50).
+(* The types A and B are reducibly convertible in Γ at level 0, given the proof R that A is reducible *)
+Reserved Notation "[ Γ ||-<0>  A ≅ B | R ]" (at level 0, Γ, A, B, R at level 50).
+(* The term t is reducible at type A and level 0 in Γ, given the proof R that A is reducible *)
+Reserved Notation "[ Γ ||-<0>  t : A | R ]" (at level 0, Γ, t, A, R at level 50).
+(* The terms t and u are reducibly convertible at type A and level 0 in Γ, given the proof R that A is reducible *)
+Reserved Notation "[ Γ ||-<0> t ≅ u : A | R ]" (at level 0, Γ, t, u, A, R at level 50).
+
 
 
 
